```{r,echo=FALSE}
options(scipen=99)
while(T){
  g1 = sample(2:9,1)
  r = sample(2:5,1)
  n = sample(6:9,1)
  gn = g1*r^(n-1)
  if(g1!=r && g1!=n && g1!=(n-1) && r!=(n-1)){break}
}
```


Question
========

A [geometric sequence](https://en.wikipedia.org/wiki/Geometric_progression) has a common **ratio** between subsequent terms (*remember an arithmetic progression has a common **difference** between terms*).

Let $g_{n}$ represent the $n$th value in a geometric progression with the following [recursive](https://en.wikipedia.org/wiki/Recurrence_relation) definition:
$$g_1 = `r g1`$$
$$g_{[n+1]} = g_{[n]}\cdot `r r`$$
where $n$ is any [natural number](https://en.wikipedia.org/wiki/Natural_number). Using this recursive definition can produce the next few values.
$$g_2 ~=~ g_1 \cdot `r r` ~=~ `r g1`\cdot`r r` ~=~ `r g1*r`$$
$$g_3 ~=~ g_2 \cdot `r r` ~=~ `r g1*r`\cdot`r r` ~=~ `r g1*r^2`$$
$$g_4 ~=~ g_3 \cdot `r r` ~=~ `r g1*r^2`\cdot`r r` ~=~ `r g1*r^3`$$

In general, if a geometric progression has an initial term $g_1$ and a common ratio $r$, we can write an explicit formula to find the $n$th value.

$$g_n = g_1r^{n-1} $$

We can solve this formula for $n$.

$$n = \frac{\log\left(\frac{g_n}{g_1}\right)}{\log(r)}+1 $$


* Evaluate $n$ such that $g_n = `r gn`$
 

Solution
========

Use the explicit formula.

$$g_n = g_1r^{n-1} $$

$$g_{`r n`} = (`r g1`)(`r r`)^{`r n`-1} $$

$$g_{`r n`} = (`r g1`)(`r r`)^{`r n-1`} $$

$$g_{`r n`} = (`r g1`)(`r r^(n-1)`) $$


$$g_{`r n`} = `r g1*r^(n-1)` $$


Meta-information
============
extype: num
exsolution: 1
exname: geometric_value_from_index