```{r,echo=F}
while(T){
  sel = sample(2:12,2)
  b = sel[1]
  x = sel[2]
  p = b^x
  if(length(unique(c(b,x,p)))==3 && x^b != p && p<10000){break}
}

ops = sort(c(b,x,p))
sol1 = paste0(1*(ops==b),collapse="")
sol2 = paste0(1*(ops==p),collapse="")
sol3 = paste0(1*(ops==x),collapse="")

al = paste0("* ",ops,"\n",collapse="")
```

Question
========

You can verify the exponential relationship below.
$$`r b`^{`r x`} = `r p`$$

These same three numbers can be used to satisfy the following logarithmic equation.

$$\log_{a}(b) = c$$

Determine values for $a$, $b$, and $c$.

* $a =$ ##ANSWER1##
* $b =$ ##ANSWER2##
* $c =$ ##ANSWER3##

Answerlist
--------

`r al`
`r al`
`r al`


Solution
========

Personally, I prefer thinking this through algebraically. We can take a log of both sides.

$$\log\left(`r b`^{`r x`}\right) = \log(`r p`)$$

When the argument of a log function has an exponent, that exponent can be brought down as a factor outside the log function.

$$`r x`\cdot\log(`r b`) = \log(`r p`)$$

We can divide both sides by $\log(`r b`)$.
$$`r x` = \frac{\log(`r p`)}{\log(`r b`)}$$

Apply the change of base rule.
$$`r x` = \log_{`r b`}(`r p`)$$
Switch the sides.

$$\log_{`r b`}(`r p`) = `r x`$$

So, $a=`r b`$ and $b=`r p`$ and $c=`r x`$.



Meta-information
============
extype: cloze
exclozetype: schoice|schoice|schoice
exsolution: `r sol1`|`r sol2`|`r sol3`
exname: logarithmic_form