---
title: "Derivation of Quadratic Formula"
output: pdf_document
---

\pagenumbering{gobble}

Begin with a generalized quadratic equation in standard form.
$$ax^2+bx+c=0$$
Subtract $c$ from both sides, and divide both sides by $a$.
$$x^2+\frac{bx}{a}=\frac{-c}{a}$$
Complete the square by adding the square of half the linear coefficient to both sides of the equation.
$$x^2+\frac{bx}{a}+\left(\frac{b}{2a}\right)^2~=~\left(\frac{b}{2a}\right)^2-\frac{c}{a}$$
Factor the perfect square.
$$\left(x+\frac{b}{2a}\right)^2=\left(\frac{b}{2a}\right)^2-\frac{c}{a}$$
Simplify the right side by distributing the exponent, making common denominator, and combining fractions.
$$\left(x+\frac{b}{2a}\right)^2~=~\frac{b^2-4ac}{4a^2}$$
Undo the squaring.
$$x+\frac{b}{2a}~=~\pm\sqrt{\frac{b^2-4ac}{4a^2}}$$
Subtract $\frac{b}{2a}$ from both sides. Also distribute the radical over the division.
$$x~=~\frac{-b}{2a}\pm \frac{\sqrt{b^2-4ac}}{2a}$$
Combine the fractions.
$$x~=~\frac{-b \pm \sqrt{b^2-4ac}}{2a}$$


