---
title: "Derivation of Quadratic Formula"
output: pdf_document
---

\pagenumbering{gobble}

Begin with a generalized quadratic equation in standard form.
$$ax^2+bx+c=0$$
Subtract $c$ from both sides.
$$ax^2+bx+c-c=-c$$
Simplify left side.
$$ax^2+bx=-c$$
Divide both sides by $a$.
$$\frac{ax^2+bx}{a}=\frac{-c}{a}$$
On the left side, distribute the divisor to both terms in the numerator.
$$\frac{ax^2}{a}+\frac{bx}{a}=\frac{-c}{a}$$
Simplify the quadratic term.
$$x^2+\frac{bx}{a}=\frac{-c}{a}$$
Complete the square by adding the square of half the linear coefficient to both sides of the equation.
$$x^2+\frac{bx}{a}+\left(\frac{b}{2a}\right)^2~=~\left(\frac{b}{2a}\right)^2-\frac{c}{a}$$
Factor the perfect square.
$$\left(x+\frac{b}{2a}\right)^2=\left(\frac{b}{2a}\right)^2-\frac{c}{a}$$
On the right side, distribute the exponent to all three factors of the quotient.
$$\left(x+\frac{b}{2a}\right)^2=\frac{b^2}{4a^2}-\frac{c}{a}$$
On the right side, make a common denominator by multiplying second term by $\frac{4a}{4a}$.
$$\left(x+\frac{b}{2a}\right)^2=\frac{b^2}{4a^2}-\frac{4ac}{4a^2}$$
On right side, combine fractions.
$$\left(x+\frac{b}{2a}\right)^2~=~\frac{b^2-4ac}{4a^2}$$
Undo the squaring.
$$x+\frac{b}{2a}~=~\pm\sqrt{\frac{b^2-4ac}{4a^2}}$$
Subtract $\frac{b}{2a}$ from both sides.
$$x~=~\frac{-b}{2a}\pm\sqrt{\frac{b^2-4ac}{4a^2}}$$

Distribute the radical over the division.
$$x~=~\frac{-b}{2a}\pm\frac{\sqrt{b^2-4ac}}{\sqrt{4a^2}}$$
Simplify the denominator.
$$x~=~\frac{-b}{2a}\pm \frac{\sqrt{b^2-4ac}}{2a}$$
Combine the fractions.
$$x~=~\frac{-b \pm \sqrt{b^2-4ac}}{2a}$$


