```{r data generation, echo = FALSE, results = "hide",warning=FALSE}

# 1/(x+p)+1/(x+q)
# (2x+(p+q))/(x^2+(p+q)x+pq)

# m/(x+p)+n/(x+q)
# ((m+n)x+(np+mq))/(x^2+(p+q)x+pq)

pq = sample(2:9,2)*sample(c(-1,1),2,T)
p = pq[1]
q = pq[2]

mn = sample(2:9,2)
m = mn[1]
n = mn[2]

exp1 = paste0("\\frac{",m,"}{x+",p,"}+\\frac{",n,"}{x+",q,"}",collapse="")
exp1 = gsub("+-","-",exp1,fixed=T)

exp2 = paste0("\\frac{",m,"\\cdot (x+",q,")}{(x+",p,")(x+",q,")}+\\frac{",n,"\\cdot(x+",p,")}{(x+",q,")(x+",p,")}",collapse="")
exp2 = gsub("+-","-",exp2,fixed=T)

m1 = paste0("\\frac{x+",q,"}{x+",q,"}",collapse="")
m1 = gsub("+-","-",m1,fixed=T)
m2 = paste0("\\frac{x+",p,"}{x+",p,"}",collapse="")
m2 = gsub("+-","-",m2,fixed=T)

exp3 = paste0("\\frac{",m,"x+",m*q,"}{x^2+",p+q,"x+",p*q,"}+\\frac{",n,"x+",n*p,"}{x^2+",p+q,"x+",p*q,"}",collapse="")
exp3 = gsub("+-","-",exp3,fixed=T)

exp4 = paste0("\\frac{",m+n,"x+",m*q+n*p,"}{x^2+",p+q,"x+",p*q,"}",collapse="")
exp4 = gsub("+-","-",exp4,fixed=T)

ans = c(m+n,m*q+n*p,p+q,p*q)
rans = c(sample(1:200,3),m-n,p-q,m+p,m+q,n+p,n+q,m*q-n*p,m*n)
ach = sort(unique(c(ans,-ans,rans,-rans)))

al = paste0("* ",ach,collapse="\n")
sol1 = paste0(1*(ans[1]==ach),collapse="")
sol2 = paste0(1*(ans[2]==ach),collapse="")
sol3 = paste0(1*(ans[3]==ach),collapse="")
sol4 = paste0(1*(ans[4]==ach),collapse="")

```

Question
========

Adding rational expressions is similar to adding fractions: specifically, a common denominator can be helpful when adding rational expressions. Find the parameters $a$, $b$, $c$, and $d$ such that the [identity](https://en.wikipedia.org/wiki/Identity_(mathematics)) below is equivalent for any value of $x$.

$$`r exp1` ~\equiv~ \frac{ax+b}{x^2+cx+d}$$

* $a=$ ##ANSWER1##
* $b=$ ##ANSWER2##
* $c=$ ##ANSWER3##
* $d=$ ##ANSWER4##


Answerlist
--------

`r al`
`r al`
`r al`
`r al`


Solution
========

The given expression:

$$`r exp1`$$

To get a common denominator, multiply the first rational fraction by $`r m1`$ and the second rational fraction by $`r m2`$.

$$`r exp2`$$

Expand both numerators and both denominators.

$$`r exp3`$$

Now, since we have common denominators, we can add the numerators.

$$`r exp4`$$

Thus,

$$a=`r ans[1]`$$
$$b=`r ans[2]`$$
$$c=`r ans[3]`$$
$$d=`r ans[4]`$$

Meta-information
============
extype: cloze
exclozetype: 
exsolution: 
exname: circ_by_compltng_sqr