```{r,echo=FALSE}
library(reticulate)
options(scipen=999)
while(T){
  R = sample(c(-6:-1,1:6),2)
  if(abs(R[1])!=abs(R[2])){break}
}
a = 1
b = -2*R[1]
c = R[1]^2+R[2]^2
rs = c(R[1],R[1],-R[1],-R[1],R[2],R[2],-R[2],-R[2])
is = c(R[2],-R[2],R[2],-R[2],R[1],-R[1],R[1],-R[1])
cns = gsub("+-","-",paste0(rs,"+",is,"i"),fixed = TRUE)
cns = gsub("1i","i",cns)
cn1 = cns[1]
cn2 = cns[2]
cns = sample(cns)
ex = paste0("x^2+",b,"x+",c,collapse="")
ex = gsub("+-","-",ex,fixed=TRUE)
sol = paste0(1*(cns==cn1)+1*(cns==cn2),collapse="")
anli = paste0("* ",cns,"\n",collapse="")
```


Question
========

The quadratic formula says if $ax^2+bx+c=0$ then $x=\frac{-b\pm\sqrt{b^2-4ac}}{2a}$.

The [radicand](https://en.wiktionary.org/wiki/radicand) is called the [discriminant](https://en.wikipedia.org/wiki/Discriminant#Degree_2). When $b^2-4ac<0$ then the solutions are [complex](https://en.wikipedia.org/wiki/Complex_number). When a quadratic equation has complex solutions, those solutions are always [complex conjugates](https://en.wikipedia.org/wiki/Complex_conjugate).

Use the quadratic formula to solve 

$$`r ex`=0$$

*Remember:* $i=\sqrt{-1}$.

Answerlist
--------
`r anli`



Solution
========

Plug numbers into the quadratic formula.

$$x = \frac{-(`r b`)\pm\sqrt{(`r b`)^2-4(`r a`)(`r c`)}}{2(`r a`)} $$

Simplify.

$$x = \frac{`r -b` \pm \sqrt{`r b^2-4*a*c`}}{`r 2*a`}$$

$$x = \frac{`r -b` \pm `r sqrt(-b^2+4*a*c)`i}{`r 2*a`}$$

$$x = `r cn2` ~~~~~~~~\text{OR}~~~~~~~~ x=`r cn1`$$


Meta-information
============
extype: mchoice
exsolution: `r sol`
exname: quadratic_formula_complex