```{r,echo=FALSE}
a = sample(2:9,3)
b = a[1]
x = a[2]
y = a[3]
z = x+y
nums = c(x,y,z)
st = paste(nums)
unk = sample(1:3,1,F)
st[unk] = "x"
```


Question
========

Solve:

$$\frac{{`r b`}^{`r st[3]`}}{{`r b`}^{`r st[2]`}}={`r b`}^{`r st[1]`}$$

Solution
========

The relevant identity:

$$\frac{b^m}{b^n} \equiv b^{m-n}$$

It should be pretty easy to see the solution.

$$\frac{{`r b`}^{`r nums[3]`}}{{`r b`}^{`r nums[2]`}}={`r b`}^{`r nums[1]`}$$

So, $x=`r nums[unk]`$.


Meta-information
============
extype: num
exsolution: `r nums[unk]`
exname: solve_exp_product