```{r,echo=F,warning=F}
fixer = function(exp){
  exp = gsub("+-","-",exp,fixed=T)
  exp = gsub("t^0","",exp,fixed=T)
  exp = gsub("h^0","",exp,fixed=T)
  exp = gsub("t^1","t",exp,fixed=T)
  exp = gsub("h^1","h",exp,fixed=T)
  return(exp)
}

aposs = 2:10
bposs = 4:7

a = sample(aposs,1)
b = sample(bposs,1)

ex1 = fixer(paste0(a,"t^",b,collapse=""))

pt = list(c(1,1),c(1,2,1),c(1,3,3,1),c(1,4,6,4,1),c(1,5,10,10,5,1),c(1,6,15,20,15,6,1),
          c(1,7,21,35,35,21,7,1),c(1,8,28,56,70,56,28,8,1))

ex2 = fixer(paste0("\\lim_{h\\to 0}\\frac{",a,"(t+h)^",b,"+",-a,"t^",b,"}{h}",collapse=""))

spt = character()
for(i in pt[[b]]){
  if(i==1){
    spt = c(spt,"")
  } else {
    spt = c(spt,as.character(i))
  }
}
bex = fixer(paste0(spt,"t^",rev(0:b),"h^",0:b,collapse="+"))
ex3 = fixer(paste0("\\lim_{h\\to 0}\\frac{",a,"\\left(",bex,"\\right)+",-a,"t^",b,"}{h}",collapse=""))
bex = fixer(paste0(a*pt[[b]],"t^",rev(0:b),"h^",0:b,collapse="+"))
ex4 = fixer(paste0("\\lim_{h\\to 0}\\frac{",bex,"+",-a,"t^",b,"}{h}",collapse=""))
bex = fixer(paste0(a*pt[[b]][2:(b+1)],"t^",rev(0:(b-1)),"h^",1:b,collapse="+"))
ex5 = fixer(paste0("\\lim_{h\\to 0}\\frac{",bex,"}{h}",collapse=""))
bex = fixer(paste0(a*pt[[b]][2:(b+1)],"t^",rev(0:(b-1)),"h^",0:(b-1),collapse="+"))
ex6 = fixer(paste0("\\lim_{h\\to 0}\\left(",bex,"\\right)",collapse=""))

ex7 = fixer(paste0(bex,collapse=""))
ex7 = gsub("h","(0)",ex7)

ac = sort(unique(as.numeric(outer(1:10,1:10))))
sol1 = paste0(1*(ac==a*b),collapse="")
sol2 = paste0(1*(ac==b-1),collapse="")
al = paste0("* ",ac,collapse="\n")

```

Question
========

Let $f(t)=`r ex1`$. The [derivative](https://en.wikipedia.org/wiki/Derivative) can be defined with a limit.

$$f'(t) ~=~ \lim_{h\to 0}\frac{f(t+h)-f(t)}{h}$$

You can prove that $f'(t)=at^b$. What are $a$ and $b$?

* $a=$ ##ANSWER1##
* $b=$ ##ANSWER2##

Answerlist
--------

`r al`
`r al`


Solution
========

We were given $f(t)$.
$$f(t)=`r ex1`$$
We were given the limit definition of a derivative.
$$f'(t) ~=~ \lim_{h\to 0}\frac{f(t+h)-f(t)}{h}$$
Use the given function in the limit definition.
$$f'(t)~=~`r ex2`$$
Use the correct [binomial expansion](https://en.wikipedia.org/wiki/Binomial_theorem).

$$f'(t)~=~`r ex3`$$

Distribute.
$$f'(t)~=~`r ex4`$$

Combine the like terms.
$$f'(t)~=~`r ex5`$$

Notice all remaining terms in numerator share a common factor of $h$, which is also in the denominator. We can eliminate this common factor.

$$f'(t)~=~`r ex6`$$

Now we can replace $h$ with $0$ (because there won't be division by 0).
$$f'(t)~=~`r ex7`$$
Simplify. Anything times 0 is 0. Anything plus 0 is that thing.

$$f'(t)~=~`r a*b`t^{`r b-1`}$$



Meta-information
============
extype: cloze
exclozetype: schoice|schoice
exsolution: `r sol1`|`r sol2`
exname: lim_def_pow