```{r,echo=FALSE}
rrr = sample(2:9,3)
b = rrr[1]
m = rrr[2]
n = rrr[3]
a = c(b,m,b,n,n,m)
s = paste(a)
u = sample(1:length(a),1)
s[u] = "x"
```


Question
========

Solve:

$$\frac{\log_{`r s[1]`}(`r s[2]`)}{\log_{`r s[3]`}(`r s[4]`)} ~=~ \log_{`r s[5]`}(`r s[6]`)$$

Solution
========

The identity:
$$\frac{\log_a(b)}{\log_a(c)} = \log_c(b)$$

So,
$$\frac{\log_{`r a[1]`}(`r a[2]`)}{\log_{`r a[3]`}(`r a[4]`)} ~=~ \log_{`r a[5]`}(`r a[6]`)$$
And thus $x=`r a[u]`$.



Meta-information
============
extype: num
exsolution: `r a[u]`
exname: log_change_base