```{r data generation, echo = FALSE, results = "hide"}
options(scipen=99)
# y = a*b^(cx)
# log_b(y/a)/c


abc = sample(2:6,3)
a = abc[1]
b = abc[2]
c = abc[3]
ops = character()
for(aa in sort(abc)){
    for(bb in sort(abc)){
        for(cc in sort(abc)){
            op = paste0("x=\\frac{\\log_{",aa,"}\\left(\\frac{y}{",bb,"}\\right)}{",cc,"}",collapse="")
            if(aa!=bb && aa!=cc && bb!=cc){
                ops = c(op,ops)
            }
        }
    }
}
ops = sample(ops)

corr = paste0("x=\\frac{\\log_{",b,"}\\left(\\frac{y}{",a,"}\\right)}{",c,"}",collapse="")

sol = paste0(1*(ops==corr),collapse="")

```


Question
========

Consider the exponential equation below. 

$$y~=~`r a`\cdot `r b`^{`r c`x}$$

Solve for $x$.

Answerlist
--------

`r paste0("* $",ops,"$",collapse="\n")`



Solution
========

Start with the given equation.

$$y~=~`r a`\cdot `r b`^{`r c`x}$$

Divide both sides by `r a`. (Division is the inverse of multiplication.)


$$\frac{y}{`r a`}~=~\frac{`r a`\cdot `r b`^{`r c`x}}{`r a`}$$

Simplify the right side.

$$\frac{y}{`r a`}~=~`r b`^{`r c`x}$$

The inverse of exponentiation with base `r b` is logarithm with base `r b`. So, we take the log, base `r b`, of both sides.


$$\log_{`r b`}\left(\frac{y}{`r a`}\right)~=~\log_{`r b`}\left(`r b`^{`r c`x}\right)$$

We know, from our [logarithm rules](https://chadworley.github.io/a2/u18/Exponent_rules.html), that $\log_B(B^z)\equiv z$. In our case, $B=`r b`$ and $z=`r c`x$. Simplify the right side. 

$$\log_{`r b`}\left(\frac{y}{`r a`}\right)~=~`r c`x$$

Divide both sides by `r c`.

$$\frac{\log_{`r b`}\left(\frac{y}{`r a`}\right)}{`r c`}~=~\frac{`r c`x}{`r c`}$$

Simplify the right side.


$$\frac{\log_{`r b`}\left(\frac{y}{`r a`}\right)}{`r c`}~=~x$$

Swap the sides to bring $x$ to the left.


$$x~=~\frac{\log_{`r b`}\left(\frac{y}{`r a`}\right)}{`r c`}$$


Meta-information
============
extype: schoice
exsolution: `r sol`
exname: solve_exponential