---
title: "Logarthmic functions are inverses of exponential functions"
output: pdf_document
---

\pagenumbering{gobble}

$$\begin{aligned}
10^4 ~&=~ 10000 &&&&\text{so}&&& \log_{10}(10000) &= 4 \\
10^3 ~&=~ 1000 &&&&\text{so}&&& \log_{10}(1000) &= 3 \\
10^2 ~&=~ 100 &&&&\text{so}&&& \log_{10}(100) &= 2 \\
10^1 ~&=~ 10 &&&&\text{so}&&& \log_{10}(10) &= 1 \\
10^0 ~&=~ 1 &&&&\text{so}&&& \log_{10}(1) &= 0 \\
10^{-1} ~&=~ 0.1 &&&&\text{so}&&& \log_{10}(0.1) &= -1 \\
10^{-2} ~&=~ 0.01 &&&&\text{so}&&& \log_{10}(0.01) &= -2 \\
10^{-3} ~&=~ 0.001 &&&&\text{so}&&& \log_{10}(0.001) &= -3 \\
10^{-4} ~&=~ 0.0001 &&&&\text{so}&&& \log_{10}(0.0001) &= -4
\end{aligned}$$

\vfill

$$\begin{aligned}
3^5 ~&=~ 243 &&&&\text{so}&&& \log_{3}(243) &= 5 \\
3^4 ~&=~ 81 &&&&\text{so}&&& \log_{3}(81) &= 4 \\
3^3 ~&=~ 27 &&&&\text{so}&&& \log_{3}(27) &= 3 \\
3^2 ~&=~ 9 &&&&\text{so}&&& \log_{3}(9) &= 2 \\
3^1 ~&=~ 3 &&&&\text{so}&&& \log_{3}(3) &= 1 \\
3^0 ~&=~ 1 &&&&\text{so}&&& \log_{3}(1) &= 0 \\\\
3^{-1} ~&=~ \frac{1}{3} &&&&\text{so}&&& \log_{3}\left(\frac{1}{3}\right) &= -1 \\\\
3^{-2} ~&=~ \frac{1}{9} &&&&\text{so}&&& \log_{3}\left(\frac{1}{9}\right) &= -2 \\\\
3^{-3} ~&=~ \frac{1}{27} &&&&\text{so}&&& \log_{3}\left(\frac{1}{27}\right) &= -3 \\\\
3^{-4} ~&=~ \frac{1}{81} &&&&\text{so}&&& \log_{3}\left(\frac{1}{81}\right) &= -4 \\\\
3^{-5} ~&=~ \frac{1}{243} &&&&\text{so}&&& \log_{3}\left(\frac{1}{243}\right) &= -5
\end{aligned}$$

$$\begin{aligned}
2^{10} ~&=~ 1024 &&&&\text{so}&&& \log_{2}(1024) &= 10 \\
2^9 ~&=~ 512 &&&&\text{so}&&& \log_{2}(512) &= 9 \\
2^8 ~&=~ 256 &&&&\text{so}&&& \log_{2}(256) &= 8 \\
2^7 ~&=~ 128 &&&&\text{so}&&& \log_{2}(128) &= 7 \\
2^6 ~&=~ 64 &&&&\text{so}&&& \log_{2}(64) &= 6 \\
2^5 ~&=~ 32 &&&&\text{so}&&& \log_{2}(32) &= 5 \\
2^4 ~&=~ 16 &&&&\text{so}&&& \log_{2}(16) &= 4 \\
2^3 ~&=~ 8 &&&&\text{so}&&& \log_{2}(8) &= 3 \\
2^2 ~&=~ 4 &&&&\text{so}&&& \log_{2}(4) &= 2 \\
2^1 ~&=~ 2 &&&&\text{so}&&& \log_{2}(2) &= 1 \\
2^0 ~&=~ 1 &&&&\text{so}&&& \log_{2}(1) &= 0 \\\\
2^{-1} ~&=~ \frac{1}{2} &&&&\text{so}&&& \log_{2}\left(\frac{1}{2}\right) &= -1 \\\\
2^{-2} ~&=~ \frac{1}{4} &&&&\text{so}&&& \log_{2}\left(\frac{1}{4}\right) &= -2 \\\\
2^{-3} ~&=~ \frac{1}{8} &&&&\text{so}&&& \log_{2}\left(\frac{1}{8}\right) &= -3 \\\\
2^{-4} ~&=~ \frac{1}{16} &&&&\text{so}&&& \log_{2}\left(\frac{1}{16}\right) &= -4 \\\\
2^{-5} ~&=~ \frac{1}{32} &&&&\text{so}&&& \log_{2}\left(\frac{1}{32}\right) &= -5 \\\\
2^{-6} ~&=~ \frac{1}{64} &&&&\text{so}&&& \log_{2}\left(\frac{1}{64}\right) &= -6 \\\\
2^{-7} ~&=~ \frac{1}{128} &&&&\text{so}&&& \log_{2}\left(\frac{1}{128}\right) &= -7 \\\\
2^{-8} ~&=~ \frac{1}{256} &&&&\text{so}&&& \log_{2}\left(\frac{1}{256}\right) &= -8 \\\\
2^{-9} ~&=~ \frac{1}{512} &&&&\text{so}&&& \log_{2}\left(\frac{1}{512}\right) &= -9 \\\\
2^{-10} ~&=~ \frac{1}{1024} &&&&\text{so}&&& \log_{2}\left(\frac{1}{1024}\right) &= -10
\end{aligned}$$









