```{r data generation, echo = FALSE, results = "hide"}
nums = c(sample(3:9,2))
am = "2(x+1)"
ad = "\\frac{x+1}{2}"
sm = "2(x-1)"
sd = "\\frac{x-1}{2}"
ma = "1x+2"
da = "\\frac{x}{1}+2"
ms = "1x-2"
ds = "\\frac{x}{1}-2"
qs = c(am,ad,sm,sd,ma,da,ms,ds)

wd = c("add 1 and then multiply by 2",
       "add 1 and then divide by 2",
       "subtract 1 and then multiply by 2",
       "subtract 1 and then divide by 2",
       "multiply by 1 and then add 2",
       "divide by 1 and then add 2",
       "multiply by 1 and then subtract 2",
       "divide by 1 and then subtract 2")

exn = sample(1:length(qs),8)
q = gsub("2",nums[2],gsub("1",nums[1],qs[exn]))
a = gsub("2",nums[1],gsub("1",nums[2],qs[length(qs)-exn+1]))
q2 = gsub("2",nums[1],gsub("1",nums[2],qs[exn]))
a2 = gsub("2",nums[2],gsub("1",nums[1],qs[length(qs)-exn+1]))
q = c(q,q2)
a = c(a,a2)

exp1 = gsub("2",nums[2],gsub("1",nums[1],wd[exn[1]]))
exp2 = gsub("2",nums[1],gsub("1",nums[2],wd[length(qs)-exn[1]+1]))

aran = sample(a)
ans = paste0(1*(a[1]==aran),collapse="")
al = paste0("* $f^{-1}(x)~=~",aran,"$\n",collapse="\n")
```

Question
========

Let function $f$ be defined with the algebraic formula below:
$$f(x) = `r q[1]`$$

Find an expression for the inverse function $f^{-1}$.

Answerlist
--------
`r al`


Solution
========

The original function tells us to `r exp1`.

The inverse function does the inverse operations in the reverse order, so it must `r exp2`.



$$f^{-1}(x)=`r a[1]`$$


Meta-information
============
extype: schoice
exsolution: `r ans`
exname: two-step_inverse_alg