```{r data generation, echo = FALSE, results = "hide"}
am = "(x+A)\\cdot B"
ad = "\\frac{x+A}{B}"
sm = "(x-A)\\cdot B"
sd = "\\frac{x-A}{B}"
ma = "A x+B"
da = "\\frac{x}{A}+B"
ms = "A x-B"
ds = "\\frac{x}{A}-B"
qs = c(am,ad,sm,sd,ma,da,ms,ds)

am = "(x+A)\\cdot B"
ad = "\\frac{x+A}{B}"
sm = "(x-A)\\cdot B"
sd = "\\frac{x-A}{B}"
ma = "A\\cdot x+B"
da = "\\frac{x}{A}+B"
ms = "A\\cdot x-B"
ds = "\\frac{x}{A}-B"
q2s = c(am,ad,sm,sd,ma,da,ms,ds)

exn = sample(1:length(qs),1)

while(T){
  nums = c(sample(2:9,2))
  x = sample(2:12,1)
  a = nums[1]
  b = nums[2]
  if(exn==1){
    y = b*(x+a)
  } else if(exn==2){
    y = (x+a)/b
  } else if(exn==3){
    y = (x-a)*b
  } else if(exn==4){
    y = (x-a)/b
  } else if(exn==5){
    y = a*x+b
  } else if(exn==6){
    y = x/a+b
  } else if(exn==7){
    y = a*x-b
  } else if(exn==8){
    y = x/a-b
  }
  if(y%%1==0 && abs(y)<70 && abs(y)>0 && x!=a && x!=b  && x!=y && y>1){break}
}

wd = c("add A and then multiply by B",
       "add A and then divide by B",
       "subtract A and then multiply by B",
       "subtract A and then divide by B",
       "multiply by A and then add B",
       "divide by A and then add B",
       "multiply by A and then subtract B",
       "divide by A and then subtract B")

q = gsub("B",nums[2],gsub("A",nums[1],qs[exn]))
a = gsub("x",y,gsub("B",nums[1],gsub("A",nums[2],q2s[length(qs)-exn+1])))

exp1 = gsub("B",nums[2],gsub("A",nums[1],wd[exn]))
exp2 = gsub("B",nums[1],gsub("A",nums[2],wd[length(qs)-exn+1]))

ques = paste0(y,"=",q)
```

Question
========

Solve the equation below.
$$`r ques`$$


Solution
========

We know that `r y` equals the result when we start with $x$ and then `r exp1`. In order to undo those operations, apply the inverse operations in reverse order: `r exp2`.

$$x = `r a`$$


So,

$$x=`r x`$$



Meta-information
============
extype: num
exsolution: `r x`
exname: two-step_equations