```{r,echo=FALSE}

# 0 = (x-h)^2+k
# -k = (x-h)^2

pn = function(c,d){
    cc = c[c!=0]
    dd = d[c!=0]
    p = paste0("{",cc,"}x^{",dd,"}",collapse="+")
    p = gsub("x^{0}","",p,fixed=T)
    p = gsub("x^{1}","x",p,fixed=T)
    p = gsub("+{-","-{",p,fixed=T)
    p = gsub("+{1}x","+x",p,fixed=T)
    p = gsub("-{1}x","-x",p,fixed=T)
    p = gsub("{-1}x","-x",p,fixed=T)
    p = gsub("{1}x","x",p,fixed=T)
    return(p)
}
twonums = sample(4:10,2)

nk = twonums[1]^2
snk = round(sqrt(nk))
h = twonums[2]*sample(c(-1,1),1)
x1 = h+snk
x2 = h-snk

ach = -20:20

sol1 = ach==x1
sol2 = ach==x2
sol = sol1 + sol2
sol = paste0(1*(sol!=0),collapse="")

al = paste0("* ",ach,collapse="\n")

```

Question
========

Find all solutions to the equation below:

$$(`r pn(c(1,-h),1:0)`)^2~=~`r nk`$$


Answerlist
-------

`r al`


Solution
========

Notice, because the [squaring](https://en.wikipedia.org/wiki/Square_(algebra)) function is NOT one-to-one, when we "undo" it on both sides of an equation, we need to consider multiple possibilities.

In this case, you should know that, when squared, both $`r -snk`$ and $`r snk`$ produce $`r nk`$.

$$(`r pn(c(1,-h),1:0)`)^2~=~`r nk`$$


$$`r pn(c(1,-h),1:0)`~=~\pm`r snk`$$


$$x~=~`r h`\pm`r snk`$$

So the two solutions are $x=`r x1`$ and $x=`r x2`$.




Meta-information
============
extype: mchoice
exsolution: `r sol`
exname: solve_sqr_x_eq_B